LL1/ParseTableGen.v
@@ -1,8 +1,12 @@
 Require Import List.
 
 Require Import Lib.Grammar.
+Require Import Lib.Lemmas.
+Require Import Lib.Tactics.
 
 Require Import LL1.ParseTable.
+
+Import ListNotations.
 
 Definition singletonLaMap la gamma :=
   LaMap.add la gamma (LaMap.empty (list symbol)).
@@ -22,14 +26,48 @@ Definition addEntry (x : nonterminal) (la : lookahead) (gamma : list symbol) (o 
     end
   end.
 
-Definition addProductionEntries (prod_and_la_set : production * LaSet.t)
+Definition addProductionEntries (production_and_la_set : production * LaSet.t)
                                 (o : option parse_table) :=
-  match prod_and_la_set with
+  match production_and_la_set with
   | ((x, gamma), laSet) =>
     fold_right (fun la o => addEntry x la gamma o) o (LaSet.elements laSet)
   end.
 
 Definition empty_pt := NtMap.empty (LaMap.t (list symbol)).
 
-Definition mkParseTable (prods_and_la_sets : list (production * LaSet.t)) :=
-  fold_right addProductionEntries (Some empty_pt) prods_and_la_sets.
+Definition mkParseTable (productions_with_la_sets : list (production * LaSet.t)) :=
+  fold_right addProductionEntries (Some empty_pt) productions_with_la_sets.
+
+(*
+Lemma mkParseTable_correct : 
+  forall (productions_and_la_sets : list (production * LaSet.t))
+         (tbl : parse_table),
+    -> mkParseTable productions_and_la_sets = Some tbl
+    -> forall (start : nonterminal)
+              (productions : list production),
+        productions = map fst productions_and_la_sets
+        (* productions_and_la_sets is well-formed *)
+        -> 
+       <-> parse_table_for tbl g.
+Proof.
+  intros; split.
+  - revert g tbl H.
+    induction productions_and_la_sets.
+    + (* empty list of productions and lookahead sets --
+         the grammar's productions must be empty, so mkParseTable should return 
+         an empty table *)
+      intros g tbl Hprods Hmk.
+      simpl in *.
+      inv Hmk.
+      unfold parse_table_for; split.
+      * unfold pt_minimal; intros x la gamma laMap Hnf Hlf.
+        exfalso; eapply NtMapFacts.empty_in_iff.
+        apply ntmap_find_in in Hnf; eauto.
+      * unfold pt_complete; intros x la gamma Hlf.
+        exfalso.
+        unfold lookahead_for in Hlf.
+        destruct Hlf as [Hin _].
+        rewrite Hprods in Hin; inv Hin.
+    + intros g tbl Hprods Hmk.
+      destruct a as [[x gamma] laSet].
+*)
